A spot of order theory

FreydSSA/Body/Fun/Basic.lean
@@ -35,15 +35,45 @@ theorem UBody.FWf.allEq {Γ Δ : FCtx ν (Ty α)} {t : UBody φ ν} (dt : FWf p 
     cases de.allEq de'
     rw [I]
 
-def UBody.FWf.maxTrg {Γ Δ : FCtx ν (Ty α)} {t : UBody φ ν} : FWf p Γ t Δ → FCtx ν (Ty α)
+def UBody.FWf.infTrg {Γ Δ : FCtx ν (Ty α)} {t : UBody φ ν} : FWf p Γ t Δ → FCtx ν (Ty α)
   | @nil _ _ _ _ _ Γ _ _ _ => Γ
-  | let1 _ _ dt => dt.maxTrg
-  | let2 _ _ _ dt => dt.maxTrg
+  | let1 _ _ dt => dt.infTrg
+  | let2 _ _ _ dt => dt.infTrg
 
-theorem UBody.FWf.maxTrg_wk {Γ Δ : FCtx ν (Ty α)} {t : UBody φ ν} (dt : FWf p Γ t Δ)
-  : dt.maxTrg.Wk Δ := by induction dt <;> assumption
+def UBody.FWf.toInf {Γ Δ : FCtx ν (Ty α)} {t : UBody φ ν} : (dt : FWf p Γ t Δ) → FWf p Γ t dt.infTrg
+  | nil _ _ => nil _ (FCtx.Wk.refl _)
+  | let1 _ de dt => let1 _ de dt.toInf
+  | let2 _ _ de dt => let2 _ _ de dt.toInf
 
---TODO: cmpTrg lore
+theorem UBody.FWf.infTrg_wk {Γ Δ : FCtx ν (Ty α)} {t : UBody φ ν} (dt : FWf p Γ t Δ)
+  : dt.infTrg.Wk Δ := by induction dt <;> assumption
+
+theorem UBody.FWf.infTrg_eq {Γ Δ Δ' : FCtx ν (Ty α)} {t : UBody φ ν}
+  (dt : FWf p Γ t Δ) (dt' : FWf p Γ t Δ')
+  : dt.infTrg = dt'.infTrg := by induction dt generalizing Δ' with
+  | nil => cases dt'; rfl
+  | let1 _ de _ I => cases dt' with | let1 _ de' dt' =>
+    cases de.tyEq de'
+    simp only [infTrg]; exact I dt'
+  | let2 _ _ de _ I => cases dt' with | let2 _ _ de' dt' =>
+    cases de.tyEq de'
+    simp only [infTrg]; exact I dt'
+
+theorem UBody.FWf.trgCmp {Γ Δ Δ' : FCtx ν (Ty α)} {t : UBody φ ν}
+  (dt : FWf p Γ t Δ) (dt' : FWf p Γ t Δ')
+  : Δ.Cmp Δ' := dt.infTrg_wk.cmp₂ (dt.infTrg_eq dt' ▸ dt'.infTrg_wk)
+
+theorem UBody.FWf.infTrg_wk' {Γ Δ : FCtx ν (Ty α)} {t : UBody φ ν} (dt : FWf p Γ t Δ) (dt' : FWf p Γ t Δ')
+  : dt.infTrg.Wk Δ' := dt.infTrg_eq dt' ▸ dt'.infTrg_wk
+
+def UBody.targets (Γ : FCtx ν (Ty α)) (p : Purity) (t : UBody φ ν)
+  : Set (FCtx ν (Ty α)) := λΔ => Nonempty (FWf p Γ t Δ)
+
+theorem UBody.FWf.infTrg_is_least {Γ Δ Δ' : FCtx ν (Ty α)} {t : UBody φ ν}
+  (dt : FWf p Γ t Δ) : IsLeast (t.targets Γ p) dt.infTrg := ⟨⟨dt.toInf⟩, λ_ ⟨dt'⟩ => dt.infTrg_wk' dt'⟩
+
+theorem UBody.FWf.infTrg_is_glb {Γ Δ Δ' : FCtx ν (Ty α)} {t : UBody φ ν}
+  (dt : FWf p Γ t Δ) : IsGLB (t.targets Γ p) dt.infTrg := ⟨λ_ ⟨dt'⟩ => dt.infTrg_wk' dt', λ_ hΔ => hΔ ⟨dt.toInf⟩⟩
 
 --TODO: FWf.comp
 
@@ -63,7 +93,7 @@ def UBody.FWfM.toFWf {Γ Δ : FCtx ν (Ty α)} {t : UBody φ ν} : FWfM p Γ t �
   | let1 x de dt => FWf.let1 x de dt.toFWf
   | let2 x y de dt => FWf.let2 x y de dt.toFWf
 
-def UBody.FWf.toFWfM {Γ Δ : FCtx ν (Ty α)} {t : UBody φ ν} : (dt : FWf p Γ t Δ) → FWfM p Γ t dt.maxTrg
+def UBody.FWf.toFWfM {Γ Δ : FCtx ν (Ty α)} {t : UBody φ ν} : (dt : FWf p Γ t Δ) → FWfM p Γ t dt.infTrg
   | FWf.nil _ w => FWfM.nil _ _
   | FWf.let1 x de dt => FWfM.let1 x de dt.toFWfM
   | FWf.let2 x y de dt => FWfM.let2 x y de dt.toFWfM
@@ -76,11 +106,9 @@ structure UBody.FWf' (p : Purity) (Γ : FCtx ν (Ty α)) (t : UBody φ ν) (Δ :
 def UBody.FWf'.toFWf {Γ Δ : FCtx ν (Ty α)} {t : UBody φ ν} (dt : UBody.FWf' p Γ t Δ) : FWf p Γ t Δ := dt.FWfM.toFWf.wkExit dt.wk
 
 def UBody.FWf.factor {Γ Δ : FCtx ν (Ty α)} {t : UBody φ ν} (dt : FWf p Γ t Δ) : UBody.FWf' p Γ t Δ where
-  live := dt.maxTrg
+  live := dt.infTrg
   FWfM := dt.toFWfM
-  wk := dt.maxTrg_wk
-
---TODO: min/max lore, e.g. FWf maxTrg and so on...
+  wk := dt.infTrg_wk
 
 --TODO: FWf'
 
